---
title: NFA
date: February 12, 2020
author: Dhruva Sambrani
---

## Formal Defn of an NFA

M = ( Q, Î£, Î´, q<sub>0</sub>, F )

Î´ : Q Ã— (Î£ âˆª {Ïµ}) â†’ ğ’«(Q)

An NFA N accepts a string s = w<sub>1</sub>w<sub>2</sub>w<sub>3</sub>...w<sub>n</sub> iff
âˆƒ a sequence of r<sub>0</sub>r<sub>1</sub>...r<sub>n</sub> âˆˆ Q such that
r<sub>n</sub> âˆˆ F and
r<sub>i+1</sub> âˆˆ Î´(r<sub>i</sub>, w<sub>i</sub>)

## Equivalence of NFA and DFA

**Theorem:**
L is regular iff it can be recognized by an NFA.

**Proof:**

If L is recognisable by a NFA (let) N = (Q, Î£, Î´, q<sub>0</sub>, F)

Consider the DFA,  D = (Q', Î£, Î´', q<sub>0</sub>', F') where  -

- Q' = ğ’«(Q)
- Î´' : Q' â†’ Q' and
  - Î´'(A, c) â†’ â‹ƒ E(Î´(a,c)), where
    - aâˆˆA
    - E(A) = the set of states connected to some qâˆˆA by Ïµ. Trivially, some qs map to themselves via a Ïµ.
- q<sub>0</sub>' = E(q<sub>0</sub>)
- F' = {A'âˆˆQ' | Aâˆ©F â‰  âˆ…}

If S is accepted by N iff âˆƒ r<sub>0</sub>...r<sub>n</sub> âˆˆ Q r<sub>0</sub>=q<sub>0</sub> and r<sub>i+1</sub> âˆˆ Î´(r<sub>i</sub>, w<sub>i</sub>)

âŸ¹ r<sub>i+1</sub> âˆˆ R<sub>i</sub> = E(Î´(r<sub>i</sub>, w<sub>i</sub>)) and r<sub>n</sub> âˆˆ R<sub>n</sub> âˆˆ F.
